wip on integration

crypto_proofs/uf1cma/Crypto.Symmetric.MAC.fst
@@ -12,6 +12,7 @@ module Crypto.Symmetric.MAC
 open Crypto.Symmetric.Bytes
 open Crypto.Indexing
 open Flag
+open FStar.Buffer
 
 module GS = Crypto.Symmetric.GF128.Spec
 module GF = Crypto.Symmetric.GF128
@@ -23,6 +24,8 @@ module HS = FStar.HyperStack
 
 type id = id * UInt128.t //NS: why not this definition : i:id & iv (alg i)
 let alg (i:id) = macAlg_of_id (fst i) 
+
+#set-options "--z3rlimit 20 --initial_fuel 1 --max_fuel 1"
 
 type text = Seq.seq (lbytes 16) // Used to be seq elem, then seq (lbytes 16)
 
@@ -60,12 +63,12 @@ let zero i : elem i =
 unfold inline_for_extraction 
 let limb = function
   | POLY1305 -> UInt64.t
-  | GHASH    -> UInt8.t
+  | GHASH    -> UInt128.t
 
 unfold inline_for_extraction
 let limb_length = function
   | POLY1305 ->  5
-  | GHASH    -> 16
+  | GHASH    -> 1
 
 inline_for_extraction unfold
 type buffer_of a = b:Buffer.buffer (limb a){Buffer.length b == limb_length a}
@@ -122,7 +125,7 @@ val sel_elem: h:mem -> #i:id -> b:elemB i{live h b} -> GTot (elem i)
 let sel_elem h #i b = 
   match reveal_elemB b with
   | B_POLY1305 b -> PL.sel_elem h b
-  | B_GHASH    b -> Buffer.as_seq h b
+  | B_GHASH    b -> GF.sel_elem h b
 
 val frame_norm: h0:mem -> h1:mem -> #i:id -> b:elemB i{live h1 b} -> Lemma
   (requires (norm h0 b /\
@@ -165,8 +168,11 @@ val rcreate: rgn:HH.rid{HS.is_eternal_region rgn} -> i:id -> ST (elemB i)
     ~(live h0 r) /\live h1 r))
 let rcreate rgn i =
   match alg i with
-  | POLY1305 -> B_POLY1305 (FStar.Buffer.rcreate rgn 0UL  5ul)
-  | GHASH    -> B_GHASH    (FStar.Buffer.rcreate rgn 0uy wlen)
+  | POLY1305 -> B_POLY1305 (FStar.Buffer.rcreate rgn 0UL 5ul)
+  | GHASH    -> B_GHASH    (FStar.Buffer.rcreate rgn (FStar.Int.Cast.uint64_to_uint128 0UL) 1ul)
+
+
+#reset-options "--z3rlimit 30 --initial_fuel 1 --max_fuel 1"
 
 val create: i:id -> StackInline (elemB i)
   (requires (fun h0 -> True))
@@ -177,7 +183,7 @@ val create: i:id -> StackInline (elemB i)
      sel_elem h1 r = zero i /\
      Buffer.frameOf b = HS.(h0.tip) /\ // /\ Map.domain h1.h == Map.domain h0.h
      Buffer.modifies_0 h0 h1 ))
-
+     
 let create i =
   match alg i with
   | POLY1305 -> 
@@ -188,7 +194,7 @@ let create i =
       //assert(Crypto.Symmetric.Poly1305.Bigint.norm h1 b);
       B_POLY1305 b
   | GHASH -> 
-      B_GHASH (FStar.Buffer.create 0uy 16ul)
+      B_GHASH (FStar.Buffer.create (FStar.Int.Cast.uint64_to_uint128 0UL) 1ul)
 
 // TODO: generalize length, add functional spec
 (** Encode raw bytes of static key as a field element *)
@@ -208,7 +214,8 @@ let encode_r #i b raw =
   | B_GHASH    b -> 
       //let h0 = ST.get () in
       //assert (Buffer.modifies_1 raw h0 h0); // Necessary for triggering right lemmas
-      Buffer.blit raw 0ul b 0ul 16ul
+      let i = GF.load128_be raw in
+      b.(0ul) <- i
 
 // TODO: generalize to word
 (** Encode a word of a message as a field element *)
@@ -216,7 +223,7 @@ val encode: i:id -> w:word_16 -> GTot (elem i)
 let encode i w =
   match alg i with 
   | POLY1305 -> PS.encode w
-  | GHASH    -> w //PS.pad_0 w (16 - Seq.length w)
+  | GHASH    -> GS.encode w
 
 (** Encode a word of a message as a field element in a buffer *)
 private val encodeB: i:id -> w:wordB_16 -> StackInline (elemB i)
@@ -232,16 +239,18 @@ let encodeB i w =
       PL.toField_plus_2_128 b w;
       B_POLY1305 b
   | GHASH ->
-      let b = Buffer.create 0uy 16ul in
-      let h0 = ST.get () in
-      Buffer.blit w 0ul b 0ul 16ul;
-      let h1 = ST.get () in
-      Seq.lemma_eq_intro (sel_word h0 w) (Seq.slice (Buffer.as_seq h0 w) 0 16);
-      Seq.lemma_eq_intro (Buffer.as_seq h1 b) (Seq.slice (Buffer.as_seq h1 b) 0 16);
+      //let buf = Buffer.create 0uy 16ul in
+      //let h0 = ST.get () in
+      //Buffer.blit w 0ul buf 0ul 16ul;
+      //let h1 = ST.get () in
+      //Seq.lemma_eq_intro (sel_word h0 w) (Seq.slice (Buffer.as_seq h0 w) 0 16);
+      //Seq.lemma_eq_intro (Buffer.as_seq h1 b) (Seq.slice (Buffer.as_seq h1 b) 0 16);
+      let v = GF.load128_be w in
+      let b = Buffer.create v 1ul in
       B_GHASH b
 
 (** Polynomial evaluation *)
-val poly: #i:id -> cs:text -> r:elem i -> Tot (elem i)
+noextract val poly: #i:id -> cs:text -> r:elem i -> Tot (elem i)
 let poly #i cs r =
   match alg i with 
   | POLY1305 -> PS.poly (text_to_PS_text cs) r
@@ -275,7 +284,7 @@ let field_mul #i a b =
   | GHASH    -> GS.op_Star_At a b
 
 noextract let op_Plus_At #i e1 e2 = field_add #i e1 e2
-let op_Star_At #i e1 e2 = field_mul #i e1 e2
+noextract let op_Star_At #i e1 e2 = field_mul #i e1 e2
 
 val poly_empty: #i:id -> t:text{Seq.length t == 0} -> r:elem i ->
   Lemma (poly #i t r == zero i)
@@ -333,7 +342,12 @@ let update #i r a w =
       let h3 = ST.get () in
       Crypto.Symmetric.Poly1305.Bigint.eval_eq_lemma h2 h3 a a 5
     end
-  | B_GHASH r, B_GHASH a -> GF.add_and_multiply a w r
+  | B_GHASH r, B_GHASH a -> 
+      push_frame();
+      let e = Buffer.create GF.zero_128 1ul in
+      e.(0ul) <- GF.load128_be w;
+      GF.add_and_multiply a e r;
+      pop_frame()
 
 
 let taglen = 16ul
@@ -373,7 +387,5 @@ let finish #i s a t =
   | B_GHASH    a ->
     begin
     GF.finish a s;
-    Buffer.blit a 0ul t 0ul 16ul;
-    let h1 = ST.get() in
-    Seq.lemma_eq_intro (Buffer.as_seq h1 t) (Seq.slice (Buffer.as_seq h1 t) 0 16)
+    GF.store128_be t a.(0ul)
     end
